.lake/build/ir/Modal/cpl/proof.c
@@ -14,13 +14,32 @@
 extern "C" {
 #endif
 LEAN_EXPORT lean_object* l_CPL_proof__system(lean_object*);
+LEAN_EXPORT lean_object* l_CPL_Valuation_ctorIdx___boxed(lean_object*, lean_object*, lean_object*);
 LEAN_EXPORT lean_object* l_CPL_semantics(lean_object*);
+LEAN_EXPORT lean_object* l_CPL_Valuation_ctorIdx(lean_object*, lean_object*, lean_object*);
 LEAN_EXPORT lean_object* l_CPL_proof__system(lean_object* x_1) {
 _start:
 {
 lean_object* x_2; 
 x_2 = lean_box(0);
 return x_2;
+}
+}
+LEAN_EXPORT lean_object* l_CPL_Valuation_ctorIdx(lean_object* x_1, lean_object* x_2, lean_object* x_3) {
+_start:
+{
+lean_object* x_4; 
+x_4 = lean_unsigned_to_nat(0u);
+return x_4;
+}
+}
+LEAN_EXPORT lean_object* l_CPL_Valuation_ctorIdx___boxed(lean_object* x_1, lean_object* x_2, lean_object* x_3) {
+_start:
+{
+lean_object* x_4; 
+x_4 = l_CPL_Valuation_ctorIdx(x_1, x_2, x_3);
+lean_dec_ref(x_2);
+return x_4;
 }
 }
 LEAN_EXPORT lean_object* l_CPL_semantics(lean_object* x_1) {
